sha3/proof/BlocksToTopLevel.ec
@@ -5,77 +5,56 @@ require (*--*) Blocks TopLevel.
 (* -------------------------------------------------------------------- *)
 require import Common.
 
-op chunk: bool list -> bool list list.
-
-op padlength (n : int) =
-  let n' = (n + 2) %% r in
-  if n' = 0 then 0 else r - n'.
-
-op pad (bs : bool list): block list =
-  let p = rcons (true :: mkseq (fun k => false) (padlength (size bs))) true in
-  map bits2w (chunk (bs ++ p)).
-
-op unpad (bs : block list): bool list option. (* Alley to fill in the definition *)
-
-axiom unpadK (bs : bool list): pcancel pad unpad.
-axiom padK (*?*) (bs : block list): ocancel unpad pad.
-
-op valid_lower (bs : block list) = unpad bs <> None.
-
-clone Blocks as Lower with
-  op valid <- valid_lower.
-
-clone TopLevel as Upper.
-
 (* -------------------------------------------------------------------- *)
-module UpperFun ( F : Lower.FUNCTIONALITY ) = {
+module UpperFun (F : Blocks.FUNCTIONALITY) = {
   proc init = F.init
 
   proc f(p : bool list, n : int) = {
-    var bs;
+    var xs;
 
-    bs  <@ F.f(pad p,(n + r - 1) /% r);
-    return take n (flatten (map w2bits bs));
+    xs <@ F.f(pad p, (n + r - 1) /% r);
+    return take n (flatten(map w2bits xs));
   }
 }.
 
-module LowerFun ( F: Upper.FUNCTIONALITY) = {
+module LowerFun (F : TopLevel.FUNCTIONALITY) = {
   proc init = F.init
 
-  proc f(p : block list, n : int) = {
-    var bs, m;
-    var bs' <- [];
+  proc f(xs : block list, n : int) = {
+    var cs, ds : bool list;
+    var obs : bool list option;
+    var ys : block list <- [];
 
-    m <- unpad p;
-    if (m <> None) {
-      bs  <@ F.f(oget m,n * r);
-      bs' <- map bits2w (chunk bs);
+    obs <- unpad xs;
+    if (obs <> None) {
+      cs <@ F.f(oget obs, n * r); (* size cs = n * r *)
+      ys <- (chunk cs).`1;
     }
-    return bs';
+    return ys;
   }
 }.
 
 (* -------------------------------------------------------------------- *)
 equiv ModularConstruction:
-  UpperFun(Lower.BlockSponge(Perm)).f ~ Upper.Sponge(Perm).f:
+  UpperFun(Blocks.BlockSponge(Perm)).f ~ TopLevel.Sponge(Perm).f:
     ={glob Perm, arg} ==> ={glob Perm, res}.
 proof.
-  proc. inline Lower.BlockSponge(Perm).f.
+  proc. inline Blocks.BlockSponge(Perm).f.
   admit. (* done *)
 qed.
 
-module ModularSimulator (S : Lower.SIMULATOR, F : Upper.FUNCTIONALITY) = S(LowerFun(F)).
+module ModularSimulator (S : Blocks.SIMULATOR, F : TopLevel.FUNCTIONALITY) = S(LowerFun(F)).
 
-module LowerDist ( D : Upper.DISTINGUISHER, F : Lower.FUNCTIONALITY, P : PRIMITIVE) =
+module BlocksDist ( D : TopLevel.DISTINGUISHER, F : Blocks.FUNCTIONALITY, P : PRIMITIVE) =
   D(UpperFun(F),P).
 
 section.
-  declare module LowerSim : Lower.SIMULATOR.
-  declare module UpperDist : Upper.DISTINGUISHER.
+  declare module BlocksSim : Blocks.SIMULATOR.
+  declare module TopLevelDist : TopLevel.DISTINGUISHER.
 
   lemma Conclusion &m:
-    `|Pr[Upper.RealIndif(Upper.Sponge,Perm,UpperDist).main() @ &m: res]
-      - Pr[Upper.IdealIndif(Upper.BIRO.IRO',ModularSimulator(LowerSim),UpperDist).main() @ &m: res]|
-    = `|Pr[Lower.RealIndif(Lower.BlockSponge,Perm,LowerDist(UpperDist)).main() @ &m: res]
-      - Pr[Lower.IdealIndif(Lower.BIRO.IRO',LowerSim,LowerDist(UpperDist)).main() @ &m: res]|.
+    `|Pr[TopLevel.RealIndif(TopLevel.Sponge,Perm,TopLevelDist).main() @ &m: res]
+      - Pr[TopLevel.IdealIndif(TopLevel.BIRO.IRO',ModularSimulator(BlocksSim),TopLevelDist).main() @ &m: res]|
+    = `|Pr[Blocks.RealIndif(Blocks.BlockSponge,Perm,BlocksDist(TopLevelDist)).main() @ &m: res]
+      - Pr[Blocks.IdealIndif(Blocks.BIRO.IRO',BlocksSim,BlocksDist(TopLevelDist)).main() @ &m: res]|.
   proof. admit. qed.
